Added some basic facts for using Kami tactics

processors/Fetch.v
@@ -32,22 +32,22 @@ Section Processor.
     Definition BtbUpdateStr :=
       STRUCT { "curPc" :: Bit addrSize; "nextPc" :: Bit addrSize }.
 
-    Definition btbPredPc := MethodSig "predPc"(Bit addrSize): Bit addrSize.
-    Definition btbUpdate := MethodSig "update"(Struct BtbUpdateStr): Void.
+    Definition btbPredPc := MethodSig "btbPredPc"(Bit addrSize): Bit addrSize.
+    Definition btbUpdate := MethodSig "btbUpdate"(Struct BtbUpdateStr): Void.
 
     Definition btb :=
       MODULE {
-          Register "targets" : Vector (Bit addrSize) indexSize <- Default
-          with Register "tags" : Vector (Bit tagSize) indexSize <- Default
-          with Register "valid" : Vector Bool indexSize <- Default
+          Register "btbTargets" : Vector (Bit addrSize) indexSize <- Default
+          with Register "btbTags" : Vector (Bit tagSize) indexSize <- Default
+          with Register "btbValid" : Vector Bool indexSize <- Default
 
-          with Method "predPc" (pc: Bit addrSize): Bit addrSize :=
+          with Method "btbPredPc" (pc: Bit addrSize): Bit addrSize :=
             LET index <- getIndex pc;
             LET tag <- getTag pc;
 
-            Read targets <- "targets";
-            Read valid <- "valid";
-            Read tags <- "tags";
+            Read targets <- "btbTargets";
+            Read valid <- "btbValid";
+            Read tags <- "btbTags";
 
             If (#valid@[#index] && (#tag == #tags@[#index]))
             then Ret #targets@[#index]
@@ -56,25 +56,25 @@ Section Processor.
             
             Ret #npc
                 
-          with Method "update" (upd: Struct BtbUpdateStr): Void :=
+          with Method "btbUpdate" (upd: Struct BtbUpdateStr): Void :=
             LET curPc <- #upd ! BtbUpdateStr @."curPc";
             LET nextPc <- #upd ! BtbUpdateStr @."nextPc";
             LET index <- getIndex curPc;
             LET tag <- getTag curPc;
 
-            Read targets: Vector (Bit addrSize) indexSize <- "targets";
-            Read valid: Vector Bool indexSize <- "valid";
-            Read tags: Vector (Bit tagSize) indexSize <- "tags";
+            Read targets: Vector (Bit addrSize) indexSize <- "btbTargets";
+            Read valid: Vector Bool indexSize <- "btbValid";
+            Read tags: Vector (Bit tagSize) indexSize <- "btbTags";
 
             If (#nextPc != (#curPc + $4))
             then
-              Write "valid" <- #valid@[#index <- $$true];
-              Write "tags" <- #tags@[#index <- #tag];
-              Write "targets" <- #targets@[#index <- #nextPc];
+              Write "btbValid" <- #valid@[#index <- $$true];
+              Write "btbTags" <- #tags@[#index <- #tag];
+              Write "btbTargets" <- #targets@[#index <- #nextPc];
               Retv
             else
               If (#tag == #tags@[#index])
-              then Write "valid" <- #valid@[#index <- $$false]; Retv;
+              then Write "btbValid" <- #valid@[#index <- $$false]; Retv;
               Retv;
             Retv
       }.
@@ -88,24 +88,24 @@ Section Processor.
       STRUCT { "pc" :: Bit addrSize; "nextPc" :: Bit addrSize }.
     Definition RedirectK := Struct (Maybe (Struct redirectStr)).
 
-    Definition redirGet := MethodSig (redirName -- "get")(): RedirectK.
-    Definition redirSetInvalid := MethodSig (redirName -- "setInvalid")(): Void.
-    Definition redirSetValid := MethodSig (redirName -- "setValid")(Struct redirectStr): Void.
+    Definition redirGet := MethodSig (redirName -- "redirGet")(): RedirectK.
+    Definition redirSetInvalid := MethodSig (redirName -- "redirSetInvalid")(): Void.
+    Definition redirSetValid := MethodSig (redirName -- "redirSetValid")(Struct redirectStr): Void.
 
     Definition redirect :=
       MODULE {
           Register redirName : RedirectK <- Default
 
-          with Method (redirName -- "get") (): RedirectK :=
+          with Method (redirName -- "redirGet") (): RedirectK :=
             Read redir <- redirName;
             Ret #redir
 
-          with Method (redirName -- "setInvalid") (): Void :=
+          with Method (redirName -- "redirSetInvalid") (): Void :=
             Write redirName: RedirectK <- STRUCT { "isValid" ::= $$false;
                                                    "value" ::= $$Default };
             Retv
 
-          with Method (redirName -- "setValid")(v: Struct redirectStr): Void :=
+          with Method (redirName -- "redirSetValid")(v: Struct redirectStr): Void :=
             Write redirName: RedirectK <- STRUCT { "isValid" ::= $$true;
                                                    "value" ::= #v };
             Retv
@@ -113,27 +113,60 @@ Section Processor.
 
   End Redirect.
 
-  Section Epoch.
-    Variable epochName: string.
+  Section DecEpoch.
+    Definition decGetEpoch1 := MethodSig "decGetEpoch1"() : Bool.
+    Definition decGetEpoch2 := MethodSig "decGetEpoch2"() : Bool.
+    Definition decToggleEpoch := MethodSig "decToggleEpoch"() : Void.
 
-    Definition getEpoch := MethodSig (epochName -- "getEpoch")() : Bool.
-    Definition toggleEpoch := MethodSig (epochName -- "toggleEpoch")() : Void.
-
-    Definition epoch :=
+    Definition decEpoch :=
       MODULE {
-        Register epochName : Bool <- false
+        Register "decEpoch" : Bool <- false
 
-        with Method (epochName -- "getEpoch") () : Bool :=
-          Read epoch <- epochName;
+        with Method "decGetEpoch1" () : Bool :=
+          Read epoch <- "decEpoch";
           Ret #epoch
 
-        with Method (epochName -- "toggleEpoch") () : Void :=
-          Read epoch <- epochName;
-          Write epochName <- !#epoch;
+        with Method "decGetEpoch2" () : Bool :=
+          Read epoch <- "decEpoch";
+          Ret #epoch
+
+        with Method "decToggleEpoch" () : Void :=
+          Read epoch <- "decEpoch";
+          Write "decEpoch" <- !#epoch;
           Retv
       }.
 
-  End Epoch.
+  End DecEpoch.
+
+  Section ExeEpoch.
+    Definition exeGetEpoch1 := MethodSig "exeGetEpoch1"() : Bool.
+    Definition exeGetEpoch2 := MethodSig "exeGetEpoch2"() : Bool.
+    Definition exeGetEpoch3 := MethodSig "exeGetEpoch3"() : Bool.
+    Definition exeToggleEpoch := MethodSig "exeToggleEpoch"() : Void.
+
+    Definition exeEpoch :=
+      MODULE {
+        Register "exeEpoch" : Bool <- false
+
+        with Method "exeGetEpoch1" () : Bool :=
+          Read epoch <- "exeEpoch";
+          Ret #epoch
+
+        with Method "exeGetEpoch2" () : Bool :=
+          Read epoch <- "exeEpoch";
+          Ret #epoch
+
+        with Method "exeGetEpoch3" () : Bool :=
+          Read epoch <- "exeEpoch";
+          Ret #epoch
+
+        with Method "exeToggleEpoch" () : Void :=
+          Read epoch <- "exeEpoch";
+          Write "exeEpoch" <- !#epoch;
+          Retv
+      }.
+
+  End ExeEpoch.
 
   Section Fetch.
     Variable (f2iName: string).
@@ -158,8 +191,8 @@ Section Processor.
           Read pc <- "pc";
           Call predPc <- btbPredPc(#pc);
           Write "pc" <- #predPc;
-          Call decEpoch <- (getEpoch "dec")();
-          Call exeEpoch <- (getEpoch "exe")();
+          Call decEpoch <- decGetEpoch1();
+          Call exeEpoch <- exeGetEpoch1();
           Call f2iEnq (
                  STRUCT { "f2dOrig" ::= STRUCT { "pc" ::= #pc;
                                                  "predPc" ::= #predPc;
@@ -179,7 +212,7 @@ Section Processor.
             Write "pc" <- #r!redirectStr@."nextPc";
             Call btbUpdate(STRUCT { "curPc" ::= #r!redirectStr@."pc";
                                     "nextPc" ::= #r!redirectStr@."nextPc" });
-            Call (toggleEpoch "exe")();
+            Call exeToggleEpoch();
             Retv
           else
             Call decRedir <- (redirGet "dec")();
@@ -189,7 +222,7 @@ Section Processor.
               Write "pc" <- #r!redirectStr@."nextPc";
               Call btbUpdate(STRUCT { "curPc" ::= #r!redirectStr@."pc";
                                       "nextPc" ::= #r!redirectStr@."nextPc" });
-              Call (toggleEpoch "dec")();
+              Call decToggleEpoch();
               Retv;
             Retv;
           Call (redirSetInvalid "exe")();
@@ -201,10 +234,11 @@ Section Processor.
 
 End Processor.
 
-Hint Unfold btb redirect epoch fetch : ModuleDefs.
+Hint Unfold btb redirect decEpoch exeEpoch fetch : ModuleDefs.
 Hint Unfold getIndex getTag BtbUpdateStr btbPredPc btbUpdate
      redirectStr RedirectK redirGet redirSetInvalid redirSetValid
-     getEpoch toggleEpoch
+     decGetEpoch1 decGetEpoch2 decToggleEpoch
+     exeGetEpoch1 exeGetEpoch2 exeGetEpoch3 exeToggleEpoch
      F2D F2I f2iEnq : MethDefs.
 
 Section Wf.
@@ -220,15 +254,40 @@ Section Wf.
     forall redirName, ModPhoasWf (redirect addrSize redirName).
   Proof. kequiv. Qed.
 
-  Lemma epoch_ModEquiv:
-    forall epochName, ModPhoasWf (epoch epochName).
+  Lemma decEpoch_ModEquiv:
+    ModPhoasWf decEpoch.
+  Proof. kequiv. Qed.
+
+  Lemma exeEpoch_ModEquiv:
+    ModPhoasWf exeEpoch.
   Proof. kequiv. Qed.
 
   Lemma fetch_ModEquiv:
     forall f2iName, ModPhoasWf (fetch addrSize dataBytes f2iName).
   Proof. kequiv. Qed.
 
+  Lemma btb_ModRegsWf:
+    ModRegsWf (btb indexSize tagSize Haddr).
+  Proof. kvr. Qed.
+
+  Lemma redirect_ModRegsWf:
+    forall redirName, ModRegsWf (redirect addrSize redirName).
+  Proof. kvr. Qed.
+
+  Lemma decEpoch_ModRegsWf:
+    ModRegsWf decEpoch.
+  Proof. kvr. Qed.
+
+  Lemma exeEpoch_ModRegsWf:
+    ModRegsWf exeEpoch.
+  Proof. kvr. Qed.
+
+  Lemma fetch_ModRegsWf:
+    forall f2iName, ModRegsWf (fetch addrSize dataBytes f2iName).
+  Proof. kvr. Qed.
+
 End Wf.
 
-Hint Resolve btb_ModEquiv redirect_ModEquiv epoch_ModEquiv fetch_ModEquiv.
+Hint Resolve btb_ModEquiv redirect_ModEquiv decEpoch_ModEquiv exeEpoch_ModEquiv fetch_ModEquiv.
+Hint Resolve btb_ModRegsWf redirect_ModRegsWf decEpoch_ModRegsWf exeEpoch_ModRegsWf fetch_ModRegsWf.
 
