refinements/MergeFetchBtb.v
@@ -1,14 +1,13 @@
 Require Import Kami.
 Require Import Lib.Indexer.
 Require Import Ex.MemTypes Ex.OneEltFifo.
-Require Import Proc.AbstractIsa Proc.FetchBtb Proc.InOrderEightStage.
+Require Import Proc.AbstractIsa Proc.Fetch Proc.FetchBtb Proc.InOrderEightStage.
 
 Set Implicit Arguments.
 Open Scope string.
 
 Section Processor.
   Variables addrSize dataBytes rfIdx: nat.
-  Variables iExecName dExecName: string.
 
   Variable decodeInst: DecodeT dataBytes rfIdx.
   Variable execInst: ExecT addrSize dataBytes rfIdx.
@@ -22,7 +21,7 @@ Section Processor.
   Definition f2i := f2i addrSize dataBytes.
 
   (** IMem related *)
-  Definition iMem := iMem addrSize dataBytes iExecName.
+  Definition iMem := iMem addrSize dataBytes.
   Definition i2d := i2d addrSize dataBytes.
 
   (** Decode related *)
@@ -30,6 +29,8 @@ Section Processor.
   Definition bht := bht addrSize bhtIndexSize.
   Definition bhtTrain := bhtTrain addrSize bhtTrainSize.
   Definition d2r := d2r addrSize dataBytes rfIdx.
+
+  Definition fetchBtb := fetchBtb dataBytes btbIndexSize btbTagSize Hbtb f2iName.
 
   (** RegRead related *)
   Definition regRead := regRead addrSize dataBytes rfIdx.
@@ -46,16 +47,25 @@ Section Processor.
   Definition m2d := m2d addrSize dataBytes rfIdx.
 
   (** DMem related *)
-  Definition dMem := dMem addrSize dataBytes rfIdx dExecName.
+  Definition dMem := dMem addrSize dataBytes rfIdx.
   Definition d2w := d2w addrSize dataBytes rfIdx.
 
   Definition writeback := writeback addrSize dataBytes rfIdx.
 
   Definition inOrderEight :=
-    inOrderEight iExecName dExecName
-                 decodeInst execInst
+    inOrderEight decodeInst execInst
                  btbIndexSize btbTagSize bhtIndexSize bhtTrainSize
                  Hbtb.
+
+  Definition inOrderEight0 :=
+    (fetchBtb ++ decRedir ++ exeRedir ++ decEpoch ++ exeEpoch ++ f2i ++
+              iMem ++ i2d ++
+              decode ++ bht ++ bhtTrain ++ d2r ++
+              regRead ++ rf ++ bypass ++ r2e ++
+              execute ++ e2m ++
+              mem ++ m2d ++
+              dMem ++ d2w ++
+              writeback)%kami.
 
   Definition fetchBtbInl :=
     fetchBtbInl dataBytes btbIndexSize btbTagSize Hbtb f2iName.
@@ -70,6 +80,52 @@ Section Processor.
             mem ++ m2d ++
             dMem ++ d2w ++
             writeback)%kami.
+
+  Hint Unfold decRedir exeRedir f2i iMem i2d
+       decode bht bhtTrain d2r fetchBtb fetchBtbInl
+       regRead rf bypass r2e execute e2m mem m2d dMem d2w
+       writeback inOrderEight inOrderEight0 inOrderEight1 : ModuleDefs.
+
+  Theorem inOrderEight_inOrderEight0:
+    inOrderEight <<== inOrderEight0.
+  Proof.
+    krewrite assoc left.
+    krefl.
+  Qed.
+
+  Theorem inOrderEight0_inOrderEight1:
+    inOrderEight0 <<== inOrderEight1.
+  Proof.
+    (* TODO: below is actually [kmodularn], but need to slightly modify it. *)
+
+    (* try (unfold MethsT; rewrite <- SemFacts.idElementwiseId). *)
+    (* apply traceRefines_modular_noninteracting. *)
+
+    (* - kequiv. *)
+    (* - kequiv. *)
+    (* - kequiv. *)
+    (* - kequiv. *)
+    (* - (* TODO: add this logic to [kdisj_regs] *) *)
+    (*   unfold projT1; repeat autounfold with ModuleDefs. *)
+    (*   kdisj_regs. *)
+    (* - unfold projT1; repeat autounfold with ModuleDefs. *)
+    (*   kdisj_regs. *)
+    (* - kvr. *)
+    (* - kvr. *)
+    (* - unfold projT1; repeat autounfold with ModuleDefs. *)
+    (*   kdisj_dms. *)
+    (* - unfold projT1; repeat autounfold with ModuleDefs. *)
+    (*   kdisj_cms. *)
+    (* - unfold projT1; repeat autounfold with ModuleDefs. *)
+    (*   kdisj_dms. *)
+    (* - unfold projT1; repeat autounfold with ModuleDefs. *)
+    (*   kdisj_cms. *)
+    (* - knoninteracting. *)
+    (* - knoninteracting. *)
+    (* - apply (projT2 fetchBtbInl). *)
+    (* - krefl. *)
+    give_up.
+  Admitted.
 
 End Processor.
 
